added pair types and wrote examples for make

theories/AlmostStlc/Examples.v
@@ -1,55 +1,99 @@
 Require Export Syntax.
+Require Export Denotation.
+Require Import List.
+Import ListNotations.
+From Equations Require Import Equations Signature.
 
+
+Section fun_lift.
+Context {Γ : ctx} {MR1 MR2 MR3 : mfix_ctx}.
+Context {t1 t2 : type}.
+Definition fun_lift : term (Arrow (Arrow t1 MR2 t2) MR3 (Arrow t1 (MR1 ++ MR2) t2 ))
+                           Γ MR3.
+apply term_abs. apply term_abs.
+apply term_lift. apply term_app with (t1 := t1).
+apply term_var. apply VarS. apply VarZ.
+apply term_var. apply VarZ.
+Defined.
+
+End fun_lift.
+
+Section plus.
+Context {Γ : ctx}.
+
+Definition plus_call : call_frame := [(Nat, Arrow Nat [] Nat)].
+
+Definition plus : term (Arrow Nat [] (Arrow Nat [] Nat)) Γ [].
+apply term_abs. apply term_abs.
+apply term_mfix with (R := plus_call) (MR := [plus_call]) (x := VarZ plus_call []).
+- apply mfix_bodies_cons.
+  + eapply term_match_nat.
+    * apply term_var. apply VarZ.
+    * apply term_abs. apply term_var. apply VarZ.
+    * eapply term_app with (t1 := Arrow Nat [] Nat).
+      {
+        apply term_abs. apply term_abs.
+        apply term_app with (t1 := Nat).
+        - apply term_var. apply VarS. apply VarZ.
+        - apply term_succ. apply term_var. apply VarZ.
+      }
+      {
+        eapply term_call. apply VarZ. apply VarZ. 
+        apply term_var. apply VarZ.
+      }
+  + apply mfix_bodies_nil.
+- eapply term_app with (t1 := Nat).
+  + apply term_app with (t1 := Arrow Nat [] Nat).
+    * apply @fun_lift with (MR1 := [plus_call]).
+    * eapply term_call.
+      -- apply VarZ.
+      -- apply VarZ.
+      -- apply term_var. apply VarZ.
+  + apply term_var. apply VarS. apply VarZ.
+Defined.
+
+End plus.
 
 Section map_term.
-Context (t1 t2 : type) (R' : rec_ctx).
+Context (t1 t2 : type) (MR : mfix_ctx).
 
-Definition map_rec : rec_ctx := (List t1, List t2) :: nil.
-(* does this give the flexibility I want with map? 
-   what if I want f to be able to make R' calls?
-   is that a good idea?
-   maybe I should instead prioritize making R calls?
-   what is here right now would define map f where 
-   f in theory could make calls to map
-
-    
+Definition map_call : call_frame := (List t1, List t2) :: nil.
 
 
-   what if I made a way to merge recursion contexts
-
-   alternatively, I could consider polymorphism for the recursion contexts
-
-   maybe some of those ideas could help solve the issue of defining recursive function that
-   can be defined using map of itself
- *)
-
-(*
-
-(t1 -map_rec-> t2) -map_rec-> List t1 -map_rec-> List t2
-
-
-(t1 -R-> t2) --> List t1 -R-> List t2
-
-*)
-
-
-Definition map_body : term (List t2) (List t1 :: (Arrow t1 map_rec t2 :: nil))%list map_rec.
+(* should come up with some notations and   *)
+Definition map_body : term (List t2) (List t1 :: List t1 :: (Arrow t1 MR t2 :: nil))%list (map_call :: MR).
 eapply term_match_list.
-- eapply term_var. constructor.
+- eapply term_var. eapply VarS. eapply VarZ.
 - eapply term_nil.
 - eapply term_cons.
-  + eapply term_app.
+  + eapply term_lift with (MR1 := [map_call]).
+    eapply term_app.
     * eapply term_var. repeat constructor.
     * eapply term_var. constructor.
   + eapply term_call.
-    * constructor.
-    * eapply term_var. repeat constructor.
+    * apply VarZ.
+    * apply VarZ.
+    * eapply term_var. apply VarS. apply VarZ.
 Defined.
 
 
-
+Definition map : term (Arrow (Arrow t1 MR t2) [] (Arrow (List t1) MR (List t2))) [] [].
+eapply term_abs. eapply term_abs.
+apply term_mfix with (R := map_call) (MR := map_call :: MR) (x := VarZ map_call MR).
+- apply mfix_bodies_cons.
+  + apply map_body.
+  + apply mfix_bodies_nil.
+- eapply term_call.
+  + apply VarZ.
+  + apply VarZ.
+  + eapply term_var. eapply VarZ.
+Defined.
 End map_term.
 
+Goal False.
+set (denote_term _ _ (map Nat Nat []) tt) as e. cbn in e.
+simp denote_term in e.
+Check (denote_term _ _ (map Nat Nat []) tt).
 
 (*
 \(f : t1 =MR=> t2) (l : List t1) ->_MR  mfix (map_rec :: MR) VarZ 
