theories/AlmostStlc/Syntax.v
@@ -1,8 +1,10 @@
+
 Require Export TypedVar.
 
 Inductive type : Type :=
   | Nat : type
   | List : type -> type
+  | Pair : type -> type -> type
   | Arrow : type -> (list (list (type * type))) -> type -> type
 .
 Notation ctx := (list type).
@@ -17,9 +19,12 @@ Inductive term : type -> ctx -> mfix_ctx -> Type :=
   | term_nil t Γ MR : term (List t) Γ MR
   | term_cons t Γ MR (head : term t Γ MR) (tail : term (List t) Γ MR) : term (List t) Γ MR
   | term_var t Γ MR (x : var t Γ) : term t Γ MR
-
+  | term_succ Γ MR (en : term Nat Γ MR) : term Nat Γ MR
   | term_match_nat t Γ MR (en : term Nat Γ MR) (eZ : term t Γ MR) (eS : term t (Nat :: Γ) MR ) : term t Γ MR
   | term_match_list t1 t2 Γ MR (el : term (List t1) Γ MR ) (enil : term t2 Γ MR) (econs : term t2 (t1 :: List t1 :: Γ) MR) : term t2 Γ MR
+  | term_pair t1 t2 Γ MR (e1 : term t1 Γ MR) (e2 : term t2 Γ MR) : term (Pair t1 t2) Γ MR
+  | term_split t1 t2 t3 Γ MR (ep : term (Pair t1 t2) Γ MR) (e : term t3 (t1 :: t2 :: Γ) MR) : term t3 Γ MR
+
   (* might be some subtleties in the application rule you are not sufficiently considering *)
   | term_app t1 t2 Γ MR (e1 : term (Arrow t1 MR t2) Γ MR) (e2 : term t1 Γ MR) : term t2 Γ MR
   (* same here *)
